Hoare assignment rule

Hoare.v
@@ -1,2 +1,90 @@
 Require Export Imp.
 
+Definition Assertion := state -> Prop.
+
+Module ExAssertions.
+
+Definition as1: Assertion := fun st => st X = 3.
+Definition as2: Assertion := fun st => st X <= st Y.
+Definition as3: Assertion :=
+    fun st => st X = 3 \/ st X <= st Y.
+Definition as4: Assertion :=
+    fun st => st Z * st Z <= st X /\
+        ~ (((S (st Z)) * (S (st Z))) <= st X).
+Definition as5 : Assertion := fun st => True.
+Definition as6 : Assertion := fun st => False.
+
+Print False.
+
+Definition assert_implies (P Q : Assertion) : Prop :=
+    forall st, P st -> Q st.
+
+Notation "P ->> Q" :=
+    (assert_implies P Q) (at level 80) : hoare_spec_scope.
+Open Scope hoare_spec_scope.
+
+Notation "P <<->> Q" :=
+    (P ->> Q /\ Q ->> P) (at level 80) : hoare_spec_scope.
+
+Definition hoare_triple
+    (P : Assertion) (c : com) (Q : Assertion) : Prop :=
+    forall st st',
+        c / st || st' ->
+        P st ->
+        Q st'.
+
+Notation "{{ P }} c {{ Q }}" :=
+    (hoare_triple P c Q) (at level 90, c at next level)
+    : hoare_spec_scope.
+
+Theorem hoare_post_true: forall (P Q : Assertion) c,
+    (forall st, Q st) ->
+    {{ P }} c {{ Q }}.
+Proof.
+    intros P Q c H. unfold hoare_triple.
+    intros st st' Heval HP.
+    apply H.
+Qed.
+
+Theorem hoare_pre_false: forall (P Q : Assertion) c,
+    (forall st, ~(P st)) ->
+    {{ P }} c {{ Q }}.
+Proof.
+    intros P Q c H. unfold hoare_triple.
+    intros st st' Heval HP. apply H in HP.
+    inversion HP.
+Qed.
+
+Definition assn_sub X a P : Assertion :=
+    fun (st : state) =>
+    P (update st X (aeval st a)).
+
+Notation "P [ X |-> a ]" := (assn_sub X a P) (at level 10).
+
+Theorem hoare_asgn: forall Q X a,
+    {{ Q [X |-> a] }} (X ::= a) {{ Q }}.
+Proof.
+    intros Q X a. unfold hoare_triple.
+    intros st st' Heval HQ'.
+    inversion Heval. subst.
+    unfold assn_sub in HQ'. assumption.
+Qed.
+
+Example assn_sub_example:
+    {{ (fun st => st X = 3) [ X |-> ANum 3 ] }}
+    (X ::= ANum 3)
+    {{ fun st => st X = 3 }}.
+Proof. apply hoare_asgn. Qed.
+
+Example hoare_asgn_examples_ex1:
+    {{ (fun st => st X <= 5) [ X |-> APlus (AId X) (ANum 1) ] }}
+    (X ::= APlus (AId X) (ANum 1))
+    {{ (fun st => st X <= 5) }}.
+Proof. apply hoare_asgn. Qed.
+
+Example hoare_asgn_examples_ex2:
+    {{ (fun st => (0 <= st X /\ st X <= 5)) [ X |-> ANum 3 ] }}
+    (X ::= ANum 3)
+    {{ (fun st => (0 <= st X /\ st X <= 5)) }}.
+Proof. apply hoare_asgn. Qed.
+
